theories/logic/model.v
@@ -12,29 +12,29 @@ From reloc Require Import prelude.properness logic.spec_rules prelude.ctx_subst.
 From reloc Require Export logic.spec_ra.
 
 (** Semantic intepretation of types *)
-Record lty2 Σ := Lty2 {
-  lty2_car :> val → val → iProp Σ;
-  lty2_persistent v1 v2 : Persistent (lty2_car v1 v2)
+Record lrel Σ := LRel {
+  lrel_car :> val → val → iProp Σ;
+  lrel_persistent v1 v2 : Persistent (lrel_car v1 v2)
 }.
-Arguments Lty2 {_} _%I {_}.
-Arguments lty2_car {_} _ _ _ : simpl never.
-Bind Scope lty_scope with lty2.
-Delimit Scope lty_scope with lty2.
-Existing Instance lty2_persistent.
+Arguments LRel {_} _%I {_}.
+Arguments lrel_car {_} _ _ _ : simpl never.
+Bind Scope lty_scope with lrel.
+Delimit Scope lty_scope with lrel.
+Existing Instance lrel_persistent.
 
 (* The COFE structure on semantic types *)
-Section lty2_ofe.
+Section lrel_ofe.
   Context `{Σ : gFunctors}.
 
-  Instance lty2_equiv : Equiv (lty2 Σ) := λ A B, ∀ w1 w2, A w1 w2 ≡ B w1 w2.
-  Instance lty2_dist : Dist (lty2 Σ) := λ n A B, ∀ w1 w2, A w1 w2 ≡{n}≡ B w1 w2.
-  Lemma lty2_ofe_mixin : OfeMixin (lty2 Σ).
-  Proof. by apply (iso_ofe_mixin (lty2_car : lty2 Σ → (val -c> val -c> iProp Σ))). Qed.
-  Canonical Structure lty2C := OfeT (lty2 Σ) lty2_ofe_mixin.
+  Instance lrel_equiv : Equiv (lrel Σ) := λ A B, ∀ w1 w2, A w1 w2 ≡ B w1 w2.
+  Instance lrel_dist : Dist (lrel Σ) := λ n A B, ∀ w1 w2, A w1 w2 ≡{n}≡ B w1 w2.
+  Lemma lrel_ofe_mixin : OfeMixin (lrel Σ).
+  Proof. by apply (iso_ofe_mixin (lrel_car : lrel Σ → (val -c> val -c> iProp Σ))). Qed.
+  Canonical Structure lrelC := OfeT (lrel Σ) lrel_ofe_mixin.
 
-  Global Instance lty2_cofe : Cofe lty2C.
+  Global Instance lrel_cofe : Cofe lrelC.
   Proof.
-    apply (iso_cofe_subtype' (λ A : val -c> val -c> iProp Σ, ∀ w1 w2, Persistent (A w1 w2)) (@Lty2 _) lty2_car)=>//.
+    apply (iso_cofe_subtype' (λ A : val -c> val -c> iProp Σ, ∀ w1 w2, Persistent (A w1 w2)) (@LRel _) lrel_car)=>//.
     - apply _.
     - apply limit_preserving_forall=> w1.
       apply limit_preserving_forall=> w2.
@@ -42,25 +42,25 @@ Section lty2_ofe.
       intros n P Q HPQ. apply (HPQ w1 w2).
   Qed.
 
-  Global Instance lty2_inhabited : Inhabited (lty2 Σ) := populate (Lty2 inhabitant).
+  Global Instance lrel_inhabited : Inhabited (lrel Σ) := populate (LRel inhabitant).
 
-  Global Instance lty2_car_ne n : Proper (dist n ==> (=) ==> (=) ==> dist n) lty2_car.
+  Global Instance lrel_car_ne n : Proper (dist n ==> (=) ==> (=) ==> dist n) lrel_car.
   Proof. by intros A A' ? w1 w2 <- ? ? <-. Qed.
-  Global Instance lty2_car_proper : Proper ((≡) ==> (=) ==> (=) ==> (≡)) lty2_car.
+  Global Instance lrel_car_proper : Proper ((≡) ==> (=) ==> (=) ==> (≡)) lrel_car.
   Proof. solve_proper_from_ne. Qed.
-End lty2_ofe.
+End lrel_ofe.
 
-Arguments lty2C : clear implicits.
+Arguments lrelC : clear implicits.
 
 Section semtypes.
   Context `{relocG Σ}.
 
   Implicit Types e : expr.
   Implicit Types E : coPset.
-  Implicit Types A B : lty2 Σ.
+  Implicit Types A B : lrel Σ.
 
   Definition refines_def (E : coPset)
-           (e e' : expr) (A : lty2 Σ) : iProp Σ :=
+           (e e' : expr) (A : lrel Σ) : iProp Σ :=
     (* TODO: refactor the quantifiers *)
     (∀ ρ, spec_ctx ρ -∗ (∀ j K, j ⤇ fill K e'
         ={E,⊤}=∗ WP e {{ v, ∃ v', j ⤇ fill K (of_val v') ∗ A v v' }}))%I.
@@ -78,91 +78,91 @@ Section semtypes.
     Proper ((=) ==> (=) ==> (≡) ==> (≡)) (refines E).
   Proof. solve_proper_from_ne. Qed.
 
-  Definition lty2_unit : lty2 Σ := Lty2 (λ w1 w2, ⌜ w1 = #() ∧ w2 = #() ⌝%I).
-  Definition lty2_bool : lty2 Σ := Lty2 (λ w1 w2, ∃ b : bool, ⌜ w1 = #b ∧ w2 = #b ⌝)%I.
-  Definition lty2_int : lty2 Σ := Lty2 (λ w1 w2, ∃ n : Z, ⌜ w1 = #n ∧ w2 = #n ⌝)%I.
+  Definition lrel_unit : lrel Σ := LRel (λ w1 w2, ⌜ w1 = #() ∧ w2 = #() ⌝%I).
+  Definition lrel_bool : lrel Σ := LRel (λ w1 w2, ∃ b : bool, ⌜ w1 = #b ∧ w2 = #b ⌝)%I.
+  Definition lrel_int : lrel Σ := LRel (λ w1 w2, ∃ n : Z, ⌜ w1 = #n ∧ w2 = #n ⌝)%I.
 
-  Definition lty2_arr (A1 A2 : lty2 Σ) : lty2 Σ := Lty2 (λ w1 w2,
+  Definition lrel_arr (A1 A2 : lrel Σ) : lrel Σ := LRel (λ w1 w2,
     □ ∀ v1 v2, A1 v1 v2 -∗ refines ⊤ (App w1 v1) (App w2 v2) A2)%I.
 
-  Definition lty2_ref (A : lty2 Σ) : lty2 Σ := Lty2 (λ w1 w2,
+  Definition lrel_ref (A : lrel Σ) : lrel Σ := LRel (λ w1 w2,
     ∃ l1 l2: loc, ⌜w1 = #l1⌝ ∧ ⌜w2 = #l2⌝ ∧
       inv (relocN .@ "ref" .@ (l1,l2)) (∃ v1 v2, l1 ↦ v1 ∗ l2 ↦ₛ v2 ∗ A v1 v2))%I.
 
-  Definition lty2_prod (A B : lty2 Σ) : lty2 Σ := Lty2 (λ w1 w2,
+  Definition lrel_prod (A B : lrel Σ) : lrel Σ := LRel (λ w1 w2,
     ∃ v1 v2 v1' v2', ⌜w1 = (v1,v1')%V⌝ ∧ ⌜w2 = (v2,v2')%V⌝ ∧
         A v1 v2 ∗ B v1' v2')%I.
 
-  Definition lty2_sum (A B : lty2 Σ) : lty2 Σ := Lty2 (λ w1 w2,
+  Definition lrel_sum (A B : lrel Σ) : lrel Σ := LRel (λ w1 w2,
     ∃ v1 v2, (⌜w1 = InjLV v1⌝ ∧ ⌜w2 = InjLV v2⌝ ∧ A v1 v2)
           ∨  (⌜w1 = InjRV v1⌝ ∧ ⌜w2 = InjRV v2⌝ ∧ B v1 v2))%I.
 
-  Definition lty2_rec1 (C : lty2C Σ -n> lty2C Σ) (rec : lty2 Σ) : lty2 Σ :=
-    Lty2 (λ w1 w2, ▷ C rec w1 w2)%I.
-  Instance lty2_rec1_contractive C : Contractive (lty2_rec1 C).
+  Definition lrel_rec1 (C : lrelC Σ -n> lrelC Σ) (rec : lrel Σ) : lrel Σ :=
+    LRel (λ w1 w2, ▷ C rec w1 w2)%I.
+  Instance lrel_rec1_contractive C : Contractive (lrel_rec1 C).
   Proof.
     intros n. intros P Q HPQ.
-    unfold lty2_rec1. intros w1 w2.
+    unfold lrel_rec1. intros w1 w2.
     apply bi.later_contractive.
     destruct n; try done.
     simpl in HPQ; simpl. f_equiv. by apply C.
   Qed.
 
-  Definition lty2_rec (C : lty2C Σ -n> lty2C Σ) : lty2 Σ := fixpoint (lty2_rec1 C).
+  Definition lrel_rec (C : lrelC Σ -n> lrelC Σ) : lrel Σ := fixpoint (lrel_rec1 C).
 
-  Definition lty2_exists (C : lty2 Σ → lty2 Σ) : lty2 Σ := Lty2 (λ w1 w2,
+  Definition lrel_exists (C : lrel Σ → lrel Σ) : lrel Σ := LRel (λ w1 w2,
     ∃ A, C A w1 w2)%I.
 
-  Definition lty2_forall (C : lty2 Σ → lty2 Σ) : lty2 Σ := Lty2 (λ w1 w2,
-    □ ∀ A : lty2 Σ, (lty2_arr lty2_unit (C A))%lty2 w1 w2)%I.
+  Definition lrel_forall (C : lrel Σ → lrel Σ) : lrel Σ := LRel (λ w1 w2,
+    □ ∀ A : lrel Σ, (lrel_arr lrel_unit (C A))%lrel w1 w2)%I.
 
-  Definition lty2_true : lty2 Σ := Lty2 (λ w1 w2, True)%I.
+  Definition lrel_true : lrel Σ := LRel (λ w1 w2, True)%I.
 
-  (** The lty2 constructors are non-expansive *)
-  Global Instance lty2_prod_ne n : Proper (dist n ==> dist n ==> dist n) lty2_prod.
+  (** The lrel constructors are non-expansive *)
+  Global Instance lrel_prod_ne n : Proper (dist n ==> dist n ==> dist n) lrel_prod.
   Proof. solve_proper. Qed.
 
-  Global Instance lty2_sum_ne n : Proper (dist n ==> dist n ==> dist n) lty2_sum.
+  Global Instance lrel_sum_ne n : Proper (dist n ==> dist n ==> dist n) lrel_sum.
   Proof. solve_proper. Qed.
 
-  Global Instance lty2_arr_ne n : Proper (dist n ==> dist n ==> dist n) lty2_arr.
+  Global Instance lrel_arr_ne n : Proper (dist n ==> dist n ==> dist n) lrel_arr.
   Proof. solve_proper. Qed.
 
-  Global Instance lty2_rec_ne n : Proper (dist n ==> dist n)
-       (lty2_rec : (lty2C Σ -n> lty2C Σ) -> lty2C Σ).
+  Global Instance lrel_rec_ne n : Proper (dist n ==> dist n)
+       (lrel_rec : (lrelC Σ -n> lrelC Σ) -> lrelC Σ).
   Proof.
     intros F F' HF.
-    unfold lty2_rec, lty2_car.
+    unfold lrel_rec, lrel_car.
     apply fixpoint_ne=> X w1 w2.
-    unfold lty2_rec1, lty2_car. cbn.
+    unfold lrel_rec1, lrel_car. cbn.
     f_equiv.
-    apply lty2_car_ne; eauto.
+    apply lrel_car_ne; eauto.
   Qed.
 
-  Lemma lty_rec_unfold (C : lty2C Σ -n> lty2C Σ) : lty2_rec C ≡ lty2_rec1 C (lty2_rec C).
+  Lemma lty_rec_unfold (C : lrelC Σ -n> lrelC Σ) : lrel_rec C ≡ lrel_rec1 C (lrel_rec C).
   Proof. apply fixpoint_unfold. Qed.
 
 End semtypes.
 
 (** Nice notations *)
-Notation "()" := lty2_unit : lty_scope.
-Infix "→" := lty2_arr : lty_scope.
-Infix "*" := lty2_prod : lty_scope.
-Infix "+" := lty2_sum : lty_scope.
-Notation "'ref' A" := (lty2_ref A) : lty_scope.
+Notation "()" := lrel_unit : lty_scope.
+Infix "→" := lrel_arr : lty_scope.
+Infix "*" := lrel_prod : lty_scope.
+Infix "+" := lrel_sum : lty_scope.
+Notation "'ref' A" := (lrel_ref A) : lty_scope.
 Notation "∃ A1 .. An , C" :=
-  (lty2_exists (λ A1, .. (lty2_exists (λ An, C%lty2)) ..)) : lty_scope.
+  (lrel_exists (λ A1, .. (lrel_exists (λ An, C%lrel)) ..)) : lty_scope.
 Notation "∀ A1 .. An , C" :=
-  (lty2_forall (λ A1, .. (lty2_forall (λ An, C%lty2)) ..)) : lty_scope.
+  (lrel_forall (λ A1, .. (lrel_forall (λ An, C%lrel)) ..)) : lty_scope.
 
 Section semtypes_properties.
   Context `{relocG Σ}.
 
   (* The reference type relation is functional and injective.
      Thanks to Amin. *)
-  Lemma interp_ref_funct E (A : lty2 Σ) (l l1 l2 : loc) :
+  Lemma interp_ref_funct E (A : lrel Σ) (l l1 l2 : loc) :
     ↑relocN ⊆ E →
-    (ref A)%lty2 #l #l1 ∗ (ref A)%lty2 #l #l2
+    (ref A)%lrel #l #l1 ∗ (ref A)%lrel #l #l2
     ={E}=∗ ⌜l1 = l2⌝.
   Proof.
     iIntros (?) "[Hl1 Hl2] /=".
@@ -176,9 +176,9 @@ Section semtypes_properties.
     compute in Hfoo. eauto.
   Qed.
 
-  Lemma interp_ref_inj E (A : lty2 Σ) (l l1 l2 : loc) :
+  Lemma interp_ref_inj E (A : lrel Σ) (l l1 l2 : loc) :
     ↑relocN ⊆ E →
-    (ref A)%lty2 #l1 #l ∗ (ref A)%lty2 #l2 #l
+    (ref A)%lrel #l1 #l ∗ (ref A)%lrel #l2 #l
     ={E}=∗ ⌜l1 = l2⌝.
   Proof.
     iIntros (?) "[Hl1 Hl2] /=".
@@ -195,12 +195,12 @@ Section semtypes_properties.
 End semtypes_properties.
 
 Notation "'REL' e1 '<<' e2 '@' E ':' A" :=
-  (refines E e1%E e2%E (A)%lty2)
+  (refines E e1%E e2%E (A)%lrel)
   (at level 100, E at next level, e1, e2 at next level,
    A at level 200,
    format "'[hv' 'REL'  e1  '/' '<<'  '/  ' e2  '@'  E  :  A ']'").
 Notation "'REL' e1 '<<' e2 ':' A" :=
-  (refines ⊤ e1%E e2%E (A)%lty2)
+  (refines ⊤ e1%E e2%E (A)%lrel)
   (at level 100, e1, e2 at next level,
    A at level 200,
    format "'[hv' 'REL'  e1  '/' '<<'  '/  ' e2  :  A ']'").
@@ -268,7 +268,7 @@ Section monadic.
     by iMod ("Hf" with "HA Hs Hj") as "Hf/=".
   Qed.
 
-  Lemma refines_ret E e1 e2 v1 v2 (A : lty2 Σ) :
+  Lemma refines_ret E e1 e2 v1 v2 (A : lrel Σ) :
     IntoVal e1 v1 →
     IntoVal e2 v2 →
     (|={E,⊤}=> A v1 v2) -∗ REL e1 << e2 @ E : A.
