theories/examples/or.v
@@ -2,7 +2,7 @@
 (** (In)equational theory of erratic choice operator (`or`). *)
 From iris.proofmode Require Import tactics.
 From iris.heap_lang.lib Require Export par.
-From reloc Require Export proofmode lib.Y (* for bot *).
+From reloc Require Export reloc lib.Y (* for bot *).
 
 (** (Binary) non-determinism can be simluated with concurrency. In
 this file we derive the algebraic laws for parallel "or"/demonic
