theories/logic/derived.v
@@ -8,7 +8,7 @@ From reloc.logic Require Export model rules.
 
 Section rules.
   Context `{relocG Σ}.
-  Implicit Types A : lty2 Σ.
+  Implicit Types A : lrel Σ.
 
   Lemma refines_wand E e1 e2 A A' :
     (REL e1 << e2 @ E : A) -∗
@@ -26,7 +26,7 @@ Section rules.
     AsRecV v' f' x' eb' →
     □(∀ v1 v2 : val, □(REL of_val v1 << of_val v2 : A) -∗
       REL App v (of_val v1) << App v' (of_val v2) : A') -∗
-    REL v << v' : (A → A')%lty2.
+    REL v << v' : (A → A')%lrel.
   Proof.
     iIntros (??) "#H".
     iApply refines_arrow_val; eauto.
