theories/reloc.v
@@ -2,3 +2,4 @@ From iris.heap_lang Require Export lang notation proofmode.
 From iris.proofmode Require Export tactics.
 From reloc.logic Require Export proofmode.tactics proofmode.spec_tactics model.
 From reloc.logic Require Export rules derived compatibility.
+From reloc.typing Require Export interp soundness.
